\documentclass[unboxed]{hwset}

% info for header block in upper right hand corner
\name{Erich L Foster}
\class{Calculus I}
\duedate{Due: 23 February 2011}
\assignment{Homework 5}

\begin{document}
\begin{problem}[1.]
	If $g(x)$ is a differentiable function and assuming that $g(x) \ne 0$ show
	that
	\begin{equation*}
		\frac{d}{dx}\left[\frac{1}{g(x)}\right] = -\frac{g'(x)}{[g(x)]^2}
	\end{equation*}
	\be
	\item By using the definition of the derivative.
	\item By using the quotient rule.
	\ee
\end{problem}

\be
	\item
	\begin{solution}
		\begin{align*}
			\frac{d}{dx}\left[\frac{1}{g(x)}\right] &= \lim_{h\to 0}
				\dfrac{\frac{1}{g(x+h)} - \frac{1}{g(x)}}{h}\\
			&=\lim_{h\to 0} \dfrac{g(x) - g(x+h)}{g(x)g(x+h)h}\\
			&=\lim_{h\to 0} \dfrac{g(x) - g(x+h)}{h} \lim_{h\to 0} \frac{1}{g(x)g(x+h)}\\
			&=-\lim_{h\to 0} \dfrac{g(x+h) - g(x)}{h} \frac{1}{[g(x)]^2}\\
			&=-\frac{g'(x)}{[g(x)]^2}
		\end{align*}
	\end{solution}
	\item
	\begin{solution}
		\begin{align*}
			\frac{d}{dx}\left[\frac{1}{g(x)}\right] &= \dfrac{\frac{d}{dx}[1]g(x) -
				\frac{d}{dx}[g(x)]}{[g(x)]^2} \\ 
			&=\frac{0\cdot g(x)-g'(x)}{[g(x)]^2} \\ 
			&=-\frac{g'(x)}{[g(x)]^2} 
		\end{align*}
	\end{solution}
\ee

\begin{problem}[2.]
	Find the derivative of 
	\begin{equation*}
		f(x) = \frac{x}{1+x^2}
	\end{equation*}
	and the equation of the tangent line to $f(x)$ at the point $(3,0.3)$.
\end{problem}

\begin{solution}
	\begin{align*}
		f'(x) &= \frac{1\cdot(1+x^2) - 2x\cdot x}{(1+x^2)^2} \\
		&= \boxed{\frac{1-x^2}{(1+x^2)^2}.}
	\end{align*}
	The equation of the tangent line is given by the point slope form
	\begin{align*}
		y - y_0 &= f'(x_0)\cdot (x - x_0) \\ 
		y - 0.3 &= \frac{1-9}{(1+9)^2}\cdot (x - 3) \\ 
		y &= -\frac{8}{100}\cdot (x - 3) + 0.3\\ 
		y &= -0.08 x + 0.24 + 0.3\\ 
		&\boxed{y = -0.08 x + 0.54.} 
	\end{align*}
\end{solution}

\begin{problem}[3.] 
	Find $f'$ and $f''$ for
	\begin{equation*}
		f(x) = e^{x}(x^3 + \sqrt{x} +1)
	\end{equation*}
\end{problem}

\begin{solution}
	\begin{align*}
		f'(x) &= \frac{d}{dx}[e^x](x^3+\sqrt{x}+1) + \frac{d}{dx}[x^3+x^{1/2}+1]e^x \\
			&= \boxed{e^x(x^3+x^{1/2}+1) + (3x^2+\frac{1}{2}x^{-1/2})e^x} \\
		f''(x) &= \frac{d}{dx}[e^x](x^3+x^{1/2}+1)+\frac{d}{dx}[x^3+x^{1/2}+1]e^x +
			\frac{d}{dx}[3x^2+\frac{1}{2}x^{-1/2}]e^x +
			\frac{d}{dx}[e^x](3x^2+\frac{1}{2}x^{-1/2}) \\
		&= \boxed{e^x(x^3+x^{1/2}+1)+(3x^2+\frac{1}{2}x^{-1/2})e^x +
			(6x-\frac{1}{4}x^{-3/2})e^x + e^x(3x^2+\frac{1}{2}x^{-1/2})}
	\end{align*}
\end{solution}

\begin{problem}[4.] 
	If $f(3) = 4,\, g(3) = 2,\, f'(3) = -6, \text{ and } g'(3) = 5,$ find the
	following numbers
	\be
		\item $(fg)'(3)$
		\item $\left(\dfrac{f}{f-g}\right)'(3)$
	\ee
\end{problem}

\be
	\item
	\begin{solution}
		\begin{align*}
			(fg)'(3) &= f'(3)g(3)+g'(3)f(3) \\
			&= -6\cdot 2 + 5\cdot 4 = \boxed{8.}
		\end{align*}
	\end{solution}
	\item
	\begin{solution}
		\begin{align*}
			\left(\frac{f}{f-g}\right)'(3) &= \frac{f'(3)(f(3)-g(3)) - (f(3)-g(3))'
				f(3)}{[f(3)-g(3)]^2} \\
			&= \frac{f'(3)(f(3)-g(3)) - (f'(3) - g'(3)) f(3)}{[f(3)-g(3)]^2} \\
			&= \frac{-6\cdot(4-2) - (-6 - 5)\cdot 4}{[4-2]^2} \\
			&= \frac{-12 + 44}{4} = \boxed{8.} 
		\end{align*}
	\end{solution}
\ee

\begin{problem}[5.]
	Find $f'$ and $f''$ for
	\begin{equation*}
		f(x) = x - 3x^{1/3}
	\end{equation*}
\end{problem}

\begin{solution}
	\begin{align*}
		\boxed{f'(x) = 1 - x^{-2/3}} \\
		\boxed{f''(x) = \frac{2}{3} x^{-5/3}.}
	\end{align*}
\end{solution}

\end{document}
