\documentclass[10pt,letterpaper]{hwset}

% info for header block in upper right hand corner
\name{Erich L Foster}
\class{Calculus I}
\assignment{Homework 8}
\duedate{23 March 2011}

\begin{document}

\begin{problem}[1.]
	Find the equation of the tangent line and normal line to  
	\begin{enumerate}
		\item \sout{$y^2 + \tan x^2y = x$ at $(0,0)$.}
		\item $x^2+\left(y-\sqrt{|x|}\right)^2=3$ at $(1,1-\sqrt{2})$. 
	\end{enumerate}
\end{problem}

\begin{enumerate}
	\item 
	\item \begin{solution}
			First notice that if $x>0$ then $|x| = x$ and so we have
			\begin{align*}
				&\frac{d}{dx}\left[ x^2 + \left( y-\sqrt{x} \right)^2 \right] =
					\frac{d}{dx}[3] \\
				&2x + \frac{d\left[\left( y-\sqrt{x} \right)^2\right]}{d\left[y-
					\sqrt{x} \right]} \frac{d\left[ y - \sqrt{x}\right]}{dx} \\
				&2x + 2\left( y-\sqrt{x} \right) \left[ y' - \frac{1}{2\sqrt{x}} \right]
					= 0 \\
					&2 + 2\left( 1-\sqrt{2} - 1\right) \left[y'-\frac{1}{2}\right] = 0 \\
					&y'-\frac{1}{2} = \frac{1}{\sqrt{2}} \\
					&y' = \frac{1}{\sqrt{2}} + \frac{1}{2} \\
					&y' = \frac{\sqrt{2} + 1}{2} \Rightarrow y'_{\perp} =
						-\frac{2}{\sqrt{2}+1} = 2-2\sqrt{2}
			\end{align*}
			\begin{align*}
				&\text{Tangent Line} &\text{Normal Line} \\
				&y - y_1 = y'(x - x_1) &y - y_1 = y'_{\perp}(x - x_1) \\ 
				&y = \frac{\sqrt{2} + 1}{2} x + \frac{1}{2}  
					&y - (1 - \sqrt{2}) = (2-2\sqrt{2})(x - 1)  \\
				&y - (1 - \sqrt{2}) = \frac{\sqrt{2} + 1}{2}(x - 1)  
					&y = (2-2\sqrt{2}) x - (2-2\sqrt{2}) + (1 - \sqrt{2})  \\
				&y = \frac{\sqrt{2} + 1}{2} x - \frac{\sqrt{2} + 1}{2} + (1 -
					\sqrt{2}) 
					&\boxed{y = (2 - \sqrt{2}) x + \sqrt{2} - 1} \\
				&\boxed{y = \frac{\sqrt{2} + 1}{2} x - \frac{3\sqrt{2} - 1}{2}}. 
			\end{align*}
		\end{solution}
\end{enumerate}

\begin{problem}[2.]
	\begin{enumerate}
		\item If $y=A \sin(\ln x) + B\cos(\ln x)$, where $A$ and $B$ are constants,
			show that 
			\begin{equation*}
				x^2y''+xy'+y=0.
			\end{equation*}
		\item Find the first and second derivative of 
			\begin{equation*}
				f(x) = \tan (\ln x^2).
			\end{equation*}
	\end{enumerate}
\end{problem}

\begin{enumerate}
	\item \begin{solution}
			\begin{align*}
				y' &= \frac{d}{dx}\left[ A\sin(\ln x) + B\cos(\ln x) \right] \\ 
				&= A\frac{d\sin(\ln x)}{d\ln x}\frac{d\ln x}{dx} +
					B\frac{d\cos(\ln x)}{d\ln x}\frac{d\ln x}{dx} \\ 
				&= A\cos(\ln x)\frac{1}{x} - B\sin(\ln x)\frac{1}{x} \\ 
				&= \frac{1}{x}\left( A\cos(\ln x) - B\sin(\ln x)\right) \\ 
				y'' &= \frac{d}{dx}\left[ \frac{1}{x}\left( A\cos(\ln x) - B\sin(\ln x)
					\right)\right] \\
					&= -\frac{1}{x^2}\left( A\cos(\ln x) - B\sin(\ln x)\right) +
						\frac{1}{x^2}\left( -A\sin(\ln x) - B\cos(\ln x) \right) \\
					&= -\frac{1}{x^2}\left[ A\left(\cos(\ln x) + \sin(\ln x)\right) -
						B\left(\sin(\ln x) - \cos(\ln x) \right)\right] \\
					&\Rightarrow -A\cos(\ln x) - A\sin(\ln x) + B\sin(\ln	x) - B\cos(\ln x) \\ 
						&\qquad+ A\cos(\ln x) - B\sin(\ln x) + A\sin(\ln x) + B\cos(\ln x) =
						0 \\ 
			\end{align*}
		\end{solution}
	\item \begin{solution}
			\begin{align*}
				f'(x) &= \frac{d}{dx}\left[ \tan(\ln x^2) \right]\\
				&= \frac{d\left[ \tan(\ln x^2) \right]}{d\left[ \ln x^2 \right]}
					\frac{d\left[ \ln x^2 \right]}{d\left[ x^2 \right]}
					\frac{d\left[ x^2 \right]}{dx} \\
				&= \sec^2 (\ln x^2)\cdot \frac{1}{x^2}\cdot 2x \\
				&= \boxed{\frac{2\sec^2 (\ln x^2)}{x}}
			\end{align*}
			\begin{align*}
				f''(x) &=\frac{d}{dx} \left[ \frac{2\sec^2 (\ln x^2)}{x} \right] \\
				&= 2\dfrac{\frac{d\left[ \sec^2(\ln x^2) \right]}{d\left[ \sec(\ln x^2)
					\right]}\frac{d\left[ \sec(\ln x^2) \right]}{d\left[ \ln x^2 \right]}
					\frac{d\left[ \ln x^2 \right]}{d\left[ x^2 \right]}
					\frac{d\left[ x^2 \right]}{dx} \cdot x - \sec^2(\ln x^2)}{x^2}\\
				&= 2\dfrac{2\sec(\ln x^2)\cdot \sec(\ln x^2)\cdot \tan(\ln x^2) \cdot
					\frac{1}{x^2}\cdot 2x \cdot x - \sec^2(\ln x^2)}{x^2}\\
				&= 2\dfrac{4\sec^2(\ln x^2)\cdot \tan(\ln x^2) - \sec^2(\ln x^2)}{x^2}\\
				&= \boxed{2\sec^2(\ln x^2)\frac{4\tan(\ln x^2) - 1}{x^2}}
				\end{align*}
		\end{solution}
\end{enumerate}

\begin{problem}[3.]
 \begin{enumerate}
	 	\item Find the first and second derivative of $\ln (y^2) + \sin (x+1) =
			e^x$.
		\item Find the first derivative of $y^x = \tan x$. \\
			Hint: Notice $y^x = e^{x \ln y}$.
 \end{enumerate}
 Be sure to substitute for $y'$ when appropriate.
\end{problem}

\begin{enumerate}
	\item \begin{solution}
		\begin{align*}
			&\frac{d}{dx}\left[ \ln y^2 + \sin(x+1) \right] = \frac{d}{dx}\left[ e^x
				\right]\\
			&2\frac{d\left[\ln y\right]}{dy}\frac{dy}{dx} + \frac{d\left[ \sin(x+1)
				\right]}{d\left[ x+1 \right]}\frac{d\left[ x+1 \right]}{dx} = e^x \\
			&\frac{2}{y}y' + \cos(x+1) = e^x \\
			&\frac{2}{y}y' = e^x - \cos(x+1) \\
			&\boxed{y' = \frac{y}{2}\left( e^x - \cos(x+1) \right)}
		\end{align*}
		\begin{align*}
			&y'' = \frac{d}{dx}\left[ \frac{y}{2}\left( e^x - \cos(x+1) \right) \right]\\
			&y'' = \frac{y'}{2}\left( e^x - \cos(x+1) \right) + \frac{y}{2}\left( e^x
				- \sin(x+1) \right) \\
			&y'' = \frac{y}{4}\left( e^x - \cos(x+1) \right)\left( e^x - \cos(x+1)
				\right) + \frac{y}{2}\left( e^x - \sin(x+1) \right) \\
			&\boxed{y'' = \frac{y}{2}\left[\frac{1}{2}\left( e^x - \cos(x+1) \right)^2
				+ e^x - \sin(x+1) \right]}
		\end{align*}
	\end{solution}
	\item \begin{solution}
		\begin{align*}
			&e^{x \ln y} = \tan x \\
			&\frac{d}{dx}\left[ e^{x \ln y} \right] = \frac{d}{dx}\left[ \tan x
				\right] \\
			&\frac{d\left[ e^{x \ln y} \right]}{d\left[ x \ln y \right]}\left( \ln y +
				x\frac{d\left[ \ln y \right]}{dy}\frac{dy}{dx} \right)  = \sec^2 x\\
			& e^{x \ln y}\left( \ln y + \frac{x}{y} y' \right)  = \sec^2 x\\
			& \left( \ln y + \frac{x}{y} y' \right)  = e^{-x \ln y}\sec^2 x\\
			& \boxed{y' = \frac{y}{x} \left( e^{-x \ln y}\sec^2 x - \ln y \right)} \\
		\end{align*}<++>
	\end{solution}<++>
\end{enumerate}

\begin{problem}[4.]
	Show the definitions of the following derivatives are correct
	\begin{enumerate}
		\item $\frac{d}{dx}\left[\cos^{-1} x\right] = -\frac{1}{\sqrt{1-x^2}}$ by
			using \tbf{Theorem 4} in the book.\\
			Hint: Let $f^{-1}(x)=\cos^{-1} x$.
		\item $\frac{d}{dx}\left[a^x\right] = \ln a \cdot a^x$, where $a$ is a
			constant. \\ 
			\begin{enumerate}
				\item By using \tbf{Theorem 4} in the book. \\
					Hint: Let $f^{-1}(x)=a^x$.
				\item By using \tbf{Logarithmic Differentiation}.
			\end{enumerate}
	\end{enumerate}
\end{problem}

\begin{enumerate}
	\item	\begin{solution}
		Let $f^{-1}(x) = \cos^{-1} x$ then $f(y) = \cos y$ and by \tbf{Theorem 4} in
		the book
		\begin{align*}
			\left[ f^{-1}(x) \right]' &= \frac{1}{f'(f^{-1}(x))} \\
			&= -\frac{1}{\sin (\cos^{-1} x)} \\
			&= -\frac{1}{\sqrt{1 - \cos^2 (\cos^{-1} x)}} \\
			&= -\frac{1}{\sqrt{1 - x^2}} 
		\end{align*}
	\end{solution}
	\item \begin{enumerate}
		\item \begin{solution}
			Let $f^{-1}(x) = a^x$ then $f(y) = \frac{\ln y}{\ln a}$ and by
			\tbf{Theorem 4} in the book
			\begin{align*}
				\left[ f^{-1}(x) \right]' &= \frac{1}{f'(f^{-1}(x))} \\
				&= \frac{1}{\frac{1}{a^x \ln a}} \\
				&= a^x \ln a. 
			\end{align*}
		\end{solution}
		\item \begin{solution}
			\begin{align*}
				y &= a^x \\
				\ln y &= x \ln a \\
				\frac{d}{dx}\left[ \ln y \right] &= \frac{d}{dx}\left[ x \ln a \right] \\
				\frac{y'}{y} &= \ln a \\
				y' &= y \ln a \\
				y' &= a^x \ln a.
				\end{align*}
		\end{solution}
	\end{enumerate}
\end{enumerate}

\end{document}

